Xv6/SpecSysWait.lean
@@ -66,7 +66,7 @@ def wp_sys_wait_body {hlc : HasLC} {GF : BundledGFunctors} [MachGS hlc GF] [Xv6G
   wpNext true k.proc cpu (fun cpu' => iprop(∀ (spie spp : Bool) (R' : RegMap) (P' : UPtd)
     (rv xw : BitVec 32) (d : Nat) (cs' : ExtTreeSet GName compare),
     ⌜calleeSaved k.regs R' ∧ R' 10#5 = BitVec.signExtend 64 rv ∧ V.upt.extSz V.sz P' ∧ d ≤ 4 ∧
-      kwaitAns rv v d⌝ -∗
+      kwaitAns rv v d ∧ umMapped P' v.toNat d⌝ -∗
     waitAns rv (xstateVal xw) cs cs' V.gen (decide (v = 0#64)) pid -∗
     chFrag V.chg (procAddr j) cs' -∗
     kctx cpu' ((k.withSpie spie spp).withRegs R') -∗ pcIs cpu' (jumpPc (k.regs 1#5)) -∗
@@ -100,7 +100,7 @@ def wp_sys_wait_eb_body {hlc : HasLC} {GF : BundledGFunctors} [MachGS hlc GF] [X
   wpNext true k.proc cpu (fun cpu' => iprop(∀ (spie spp : Bool) (R' : RegMap) (P' : UPtd)
     (rv xw : BitVec 32) (d : Nat) (cs' : ExtTreeSet GName compare),
     ⌜calleeSaved k.regs R' ∧ R' 10#5 = BitVec.signExtend 64 rv ∧ V.upt.extSz V.sz P' ∧ d ≤ 4 ∧
-      kwaitAns rv v d⌝ -∗
+      kwaitAns rv v d ∧ umMapped P' v.toNat d⌝ -∗
     waitAns rv (xstateVal xw) cs cs' V.gen (decide (v = 0#64)) pid -∗
     chFrag V.chg (procAddr j) cs' -∗
     kctx cpu' ((k.withSpie spie spp).withRegs R') -∗ pcIs cpu' (jumpPc (k.regs 1#5)) -∗
